ironfleet/src/Dafny/Distributed/Common/Framework/Performance_arith.s.dfy
@@ -1,0 +1,81 @@
+include "Environment.s.dfy"
+include "Host.s.dfy"
+include "DistributedSystem.s.dfy"
+include "../Collections/Seqs.i.dfy"
+
+abstract module Performance_s {
+  import opened Collections__Seqs_i
+  import opened DS_s : DistributedSystem_s
+
+  type PerfObject = i : int | 0 <= i
+
+  function {:axiom} PerfMax(p1:PerfObject, p2:PerfObject) : PerfObject
+    // ensures PerfMax(p1, p2) >= p1 && PerfMax(p1, p2) >= p2
+    // ensures PerfMax(p1, p2) == p1 || PerfMax(p1, p2) == p2
+    ensures p1 >= p2 ==> PerfMax(p1, p2) == p1
+    ensures p2 >= p1 ==> PerfMax(p1, p2) == p2
+  {
+    if p1 < p2 then
+      p2
+    else 
+      p1
+  }
+
+  function PerfZero() : PerfObject
+  {
+    0
+  }
+
+  function PerfVoid() : PerfObject
+  {
+    0
+  }
+
+  function {:axiom} PerfDelivery() : imap<nat, PerfObject>
+    ensures imaptotal(PerfDelivery())
+
+  function {:axiom} PerfStep(hstep:HostStep) : imap<nat, PerfObject>
+    ensures imaptotal(PerfStep(hstep))
+
+  function PerfAdd2(p1:PerfObject, p2:PerfObject) : PerfObject
+  {
+    p1 + p2
+  }
+
+  type PerfExpr = PerfObject
+
+  datatype NumSteps = NumSteps(num_hsteps:imap<HostStep, nat>, num_deliveries:nat)
+    
+  predicate ValidNumSteps(num_steps:NumSteps)
+  {
+    imaptotal(num_steps.num_hsteps)
+  }
+
+  function NumStepsInit() : NumSteps
+  {
+    NumSteps(imap h:HostStep | true :: 0 as nat , 0)
+  }
+
+  function NoRecvPerfUpdate(node_pr:PerfExpr, hstep:HostStep, num_steps:NumSteps) : (PerfExpr, NumSteps)
+    requires ValidNumSteps(num_steps)
+    ensures ValidNumSteps(num_steps)
+  {
+    var step_idx := num_steps.num_hsteps[hstep];
+    var total_time := PerfAdd2(node_pr, PerfStep(hstep)[step_idx]);
+    var num_steps' := num_steps.(num_hsteps := num_steps.num_hsteps[hstep := num_steps.num_hsteps[hstep] + 1]);
+    (total_time, num_steps')
+  }
+
+  function RecvPerfUpdate(node_pr:PerfExpr, pkt_pr:PerfExpr, hstep:HostStep, num_steps:NumSteps) : (PerfExpr, NumSteps)
+    requires ValidNumSteps(num_steps)
+    ensures ValidNumSteps(num_steps)
+  {
+    var delivery_idx := num_steps.num_deliveries;
+    var deliveryTime := PerfAdd2(pkt_pr, PerfDelivery()[delivery_idx]);
+    var handlerStartTime := PerfMax(deliveryTime, node_pr);
+    var step_idx := num_steps.num_hsteps[hstep];
+    var total_time := PerfAdd2(handlerStartTime, PerfStep(hstep)[step_idx]);
+    var num_steps' := num_steps.(num_hsteps := num_steps.num_hsteps[hstep := num_steps.num_hsteps[hstep] + 1], num_deliveries := num_steps.num_deliveries + 1);
+    (total_time, num_steps')
+  }
+}
